updates

high2/Zeta.EAC.fst
@@ -5,58 +5,135 @@ open Zeta.SeqAux
 
 let eac_state_of_base_key
   (#app: app_params)
+  (k: base_key)
   (l: vlog_ext app)
-  (k: base_key): eac_state app k
+  : eac_state app k
   = seq_machine_run (eac_smk app k) l
 
 let eac_state_transition_aux
   (#app: app_params)
-  (l: vlog_ext app {length l > 0})
   (k: base_key)
+  (l: vlog_ext app {length l > 0})
   : Lemma (ensures (let open Zeta.SeqAux in
                     let n = length l - 1 in
                     let l' = prefix l n in
                     let ee = index l n in
-                    let es' = eac_state_of_base_key l' k in
-                    let es = eac_state_of_base_key l k in
+                    let es' = eac_state_of_base_key k l' in
+                    let es = eac_state_of_base_key k l in
                     es = eac_add ee es'))
-          [SMTPat (eac_state_of_base_key l k)]
-  = admit()
+          [SMTPat (eac_state_of_base_key k l)]
+  = let n = length l - 1 in
+    let l' = prefix l n in
+    let ee = index l n in
+    let smk = eac_smk app k in
+    lemma_hprefix_append_telem l;
+    lemma_reduce_append (init_state smk) (trans_fn smk) l' ee
 
 let eac_state_transition
   (#app: app_params)
-  (l: vlog_ext app {length l > 0})
   (k: key app)
+  (l: vlog_ext app {length l > 0})
   : Lemma (ensures (let open Zeta.SeqAux in
                     let n = length l - 1 in
                     let l' = prefix l n in
                     let ee = index l n in
-                    let es' = eac_state_of_key l' k in
-                    let es = eac_state_of_key l k in
+                    let es' = eac_state_of_key k l' in
+                    let es = eac_state_of_key k l in
                     es = eac_add ee es'))
-  =
-
-  admit()
+  = let bk = to_base_key k in
+    eac_state_transition_aux bk l
 
 let eac_empty_log
   (#app: app_params)
   (l: vlog_ext app {length l = 0})
   : Lemma (ensures (eac l))
           [SMTPat (eac l)]
-  = admit()
+  = lemma_empty l;
+    let aux (k: base_key)
+        : Lemma (ensures (valid (eac_smk app k) l))
+                  [SMTPat (valid (eac_smk app k) l)]
+      = lemma_empty_seq_valid (eac_smk app k)
+    in
+    ()
+
+
+let rec search_keys_subtree (f: base_key -> bool) (k: base_key)
+  : Tot (o: (option base_key)
+    {
+      o = None /\ (forall (k': base_key). Zeta.BinTree.is_desc k' k ==> f k')
+        \/
+      Some? o /\ not ( f (Some?.v o) )
+    })
+    (decreases (height k))
+    = let open Zeta.BinTree in
+      if not (f k) then Some k
+      else if height k = 0 then (
+        let aux (k':base_key)
+          : Lemma (ensures (is_desc k' k ==> f k'))
+          = if k' = k then ()
+            else if not (is_desc k' k) then ()
+            else assert(is_proper_desc k' k)
+        in
+        FStar.Classical.forall_intro aux;
+        None
+      )
+      else
+        let ol = search_keys_subtree f (LeftChild k) in
+        let or = search_keys_subtree f (RightChild k) in
+        if Some? ol then ol
+        else if Some? or then or
+        else (
+          let aux (k': base_key)
+            : Lemma (ensures (is_desc k' k ==> f k'))
+            = if k' = k then ()
+              else if not (is_desc k' k) then ()
+              else
+                let d = desc_dir k' k in
+                if d = Left then ()
+                else ()
+          in
+          FStar.Classical.forall_intro aux;
+          None
+        )
+
+(* since the space of keys is finite, we can computationally determine if a property is true for all keys
+ * or find a key if this is not the case *)
+let search_keys (f: base_key -> bool)
+  : o: (option base_key)
+    {
+      o = None /\ (forall (k: base_key). f k)
+        \/
+      Some? o /\ not (f (Some?.v o))
+    }
+  = let open Zeta.BinTree in
+    let o = search_keys_subtree f Root in
+    if None = o then (
+      let aux (k: base_key)
+        : Lemma (ensures (f k))
+                [SMTPat (f k)]
+        = lemma_root_is_univ_ancestor k
+      in
+      o
+    )
+    else o
 
 let eac_induction_step_helper
   (#app: app_params)
-  (l: vlog_ext app)
-  (i: seq_index l {eac (prefix l i)})
+  (l: vlog_ext app{let n = length l in n > 0 /\ eac (prefix l (n - 1))})
   : o: (option base_key)
-    {
-      o = None /\ eac (prefix l (i + 1))
+    {let n = length l in
+      o = None /\ eac l
           \/
-      (let k = Some?.v o in
-       eac_state_of_key (prefix l (i + 1)) k = EACFail)
+          Some? o /\
+          (let k = Some?.v o in
+           eac_state_of_base_key k l = EACFail)
     }
-  = admit()
+  = let n = length l - 1 in
+    let l' = prefix l n in
+    let ee = index l n in
+    let e = to_vlog_entry ee in
+    let f = fun (k: base_key) -> valid (eac_smk app k) l in
+    search_keys f
 
 let rec max_eac_prefix_aux
   (#app: app_params)
@@ -72,23 +149,52 @@ let rec max_eac_prefix_aux
       })
      (decreases (length l))
   = let n = length l in
-    if n = 0 then Zeta.BinTree.Root (* any key since eac*), 0
+    if n = 0 then (
+      eac_empty_log l;
+      Zeta.BinTree.Root (* the returned key is don't care for eac l *), 0
+    )
     else
-      let n = n - 1 in
-      let l' = prefix l n in
-      let ee = index l n in
-      let i' = max_eac_prefix_aux l' in
-      admit()
+      let l' = prefix l (n - 1) in
+      let k,i' = max_eac_prefix_aux l' in
+      if i' = n - 1 then
+        let o = eac_induction_step_helper l in
+        if None = o
+        then Zeta.BinTree.Root, n
+        else (
+          let k = Some?.v o in
+          let smk = eac_smk app k in
+          assert(~ (valid smk l));
+          k,n-1
+        )
+      else k,i'
 
-
-let eac_implies_prefix_eac
+let rec eac_implies_prefix_eac
   (#app: app_params)
   (l: eac_log app)
   (i: nat {i <= length l})
   : Lemma (ensures (eac (prefix l i)))
-  =
+          (decreases (length l))
+  = if i = length l then ()
+    else
+      let n = length l - 1 in
+      let l' = prefix l n in
+      let k,i' = max_eac_prefix_aux l' in
+      if i' = n
+      then
+        eac_implies_prefix_eac l' i
+      else
+        let smk = eac_smk app k in
+        lemma_valid_prefix smk l (i' + 1)
 
-  admit()
+let lemma_eac_state_of_key
+  (#app: app_params)
+  (l: eac_log app)
+  (k: key app)
+  : Lemma (ensures (eac_state_of_key k l <> EACFail))
+  = let bk = to_base_key k in
+    let smk = eac_smk app bk in
+    assert(valid smk l);
+    ()
 
 let max_eac_prefix
   (#app: app_params)
@@ -98,7 +204,8 @@ let max_eac_prefix
           i < length l /\
           eac (prefix l i) /\
           ~ (eac (prefix l (i + 1)))})
-  = admit()
+  = let _,i = max_eac_prefix_aux l in
+    i
 
 (* computable version of eac *)
 let is_eac_log (#app: app_params) (l:vlog_ext app): (r:bool{r <==> eac l})
@@ -106,3 +213,56 @@ let is_eac_log (#app: app_params) (l:vlog_ext app): (r:bool{r <==> eac l})
     if i = length l
     then true
     else false
+
+let eac_value_base (#app: app_params) (k: key app) (l: eac_log app)
+  : value app
+  = let es = eac_state_of_key k l in
+    match es with
+    | EACInit -> init_value k
+    | EACInStore _ v -> v
+    | EACEvictedMerkle v -> v
+    | EACEvictedBlum v _ _ -> v
+
+let rec lemma_eac_value_compatible (#app: app_params) (k: key app) (l: eac_log app)
+  : Lemma (ensures (Zeta.Record.compatible k (eac_value_base k l)))
+          (decreases (length l))
+          [SMTPat (eac_value_base k l)]
+  = let n = length l in
+    let bk = to_base_key k in
+    let smk = eac_smk app bk in
+    lemma_eac_state_of_key l k;
+    if n = 0 then
+      lemma_empty_seq_init smk l
+    else (
+      let l' = prefix l (n - 1) in
+      let es' = eac_state_of_base_key bk l' in
+      let ee = index l (n - 1) in
+      let e = to_vlog_entry ee in
+      lemma_eac_value_compatible k l';
+      if not (e `refs_key` bk)
+      then ()
+      else
+        match es' with
+        | EACInit -> (
+          match ee with
+          | NEvict (AddM (k2,v) _ _) -> ()
+          | _ -> ()
+        )
+        | _ -> ()
+    )
+
+let eac_value (#app: app_params) (k: key app) (l: eac_log app)
+  : value_t k
+  = eac_value_base k l
+
+let eac_implies_valid_simulation (#app: app_params) (l: eac_log app)
+  : Lemma (ensures (let fs = appfn_call_seq l in
+                    Some? (simulate fs)))
+  = admit()
+
+let eac_state_is_app_state (#app: app_params) (l: eac_log app) (k: app_key app.adm)
+  : Lemma (ensures (let fs = appfn_call_seq l in
+                    let app_state,_ = Some?.v (simulate fs) in
+                    let gk = AppK k in
+                    eac_value gk l = AppV (app_state k)))
+  = admit()
